 # 多值依赖几个定理
若$X\to \to Y$且$A\subseteq X$, 则$X\to \to YA$
> 证：
> $\forall t_1, t_2$满足$t_1\cdot X = t_2\cdot X$
> $\exists t_3$满足$t_3 \cdot XY = t_1 \cdot XY$
> $\qquad$且$t_3 \cdot(R-XY)=t_2 \cdot(R-XY)$
> 此时$t_3 \cdot XAY = t_1 \cdot XAY$
> $\qquad$且$$
\begin{aligned}
t_3\cdot (R-XAY) &= t3\cdot (R-XY) \\
&= t2\cdot (R-XY) \\
&= t2\cdot (R-XAY) \\
\end{aligned}
$$
$\therefore X\to\to AY$
---
（增补率）若$X\to\to Y$,且$W \supseteq Z$，则$XW\to\to YZ$
> 证：
> 先证：若$X\to\to Y$，则$XW\to\to Y$
> > $\forall t1, t2$满足$t_1 \cdot XW= t_1 \cdot XW$
> $\therefore t_1 \cdot X= t_1 \cdot X$
> $\because X\to\to Y$
> $\exists t_3$, 满足$t_3 \cdot XY = t_1 \cdot XY$
> $\qquad$ 且$t_3 \cdot (R-XY) = t_2 \cdot (R-XY)$
> $\because XY\cap W \subseteq XY$
> $\quad (R-XY) \cup W \subseteq (R-XY)$
> 此时
> $t_3 \cdot (XY\cup W)=t_1\cdot (XY\cup W)$
> $t_3 \cdot ((R-XY)\cup W)=t_1\cdot ((R-XY)\cup W)=t_2\cdot ((R-XY)\cup W)$
> $$
\begin{aligned}
\therefore t_3 \cdot W &= t_3 \cdot (XY\cup W) \times t_3 \cdot ((R-XY)\cup W) \\
&= t_1 \cdot (XY\cup W) \times t_1 \cdot ((R-XY)\cup W)  \\
&=t_1\cdot W
\end{aligned}$$
> $$\therefore t_3 \cdot XYW = t_1 \cdot XYW$$
> 另外，$\because R-XYW \subseteq R-XY$
> $\therefore t_3\cdot (R-XYW) = t_1\cdot (R-XYW)$
> $\therefore XW\to\to Y$
> ---
> 再证:若$X\to\to Y$,且$W \supseteq Z$，则$XW\to\to YZ$
> > 引理：若$X\to \to Y$且$A\subseteq X$, 则$X\to \to YA$
> $Z\subseteq XW$
> 显然可得
<!--stackedit_data:
eyJoaXN0b3J5IjpbLTIxNDE5MDcxNjNdfQ==
-->